Valaig/Aig.lean
@@ -8,3 +8,4 @@ public import Valaig.Aig.WellFormed
 public import Valaig.Aig.Semantics
 public import Valaig.Aig.Iter
 public import Valaig.Aig.FromStd
+public import Valaig.Aig.Projections
