Valaig/Aig/Projections.lean
@@ -1,0 +1,64 @@
+module
+
+import all Valaig.Aig.Basic
+public import Valaig.Aig.WellFormed
+public import Valaig.Aig.Iter
+
+/-
+Project out the reset and transition relation components of an Aig as new combinational Aigs.
+These may go in the future, replaced by better methods for going straight to SAT
+-/
+
+public section
+namespace Valaig.Aig
+
+def resetAig (aig : Aig) (wf : aig.WellFormed) : Aig :=
+  go aig.iter .empty (.emptyWithCapacity aig.size)
+where
+  go iter (state : Aig) (map : Array Lit)
+    (size : iter.var.idx = map.size := by grind)
+    (valid : ∀ {lit} (_ : lit ∈ map), lit.validIn state := by grind) :=
+    match h : iter.step.val with
+    | .skip it => go iter state map
+    | .done => state
+    | .yield it' var =>
+      let mapLit (lit : Lit) (h : lit.var < var := by grind) : Lit :=
+        map[lit.var.idx]'(by grind) |>.invert lit.inverted
+
+      let res : Aig × Lit := 
+        match h : aig[var]'(by grind) with
+        | .false => (state, .false)
+        | .input _ =>
+          let (eq:=_) (state, idx) := state.addInput
+          (state, idx.getLit state)
+        | .latch idx => (state, mapLit <| idx.getReset aig)
+        | .and rhs0 rhs1 => state.addAnd (mapLit rhs0) (mapLit rhs1)
+
+      go it' res.fst (map.push res.snd) (by simp; grind) (by simp [res]; grind)
+  termination_by iter.length
+  decreasing_by all_goals grind
+
+def transAig (aig : Aig) (wf : aig.WellFormed) : Aig :=
+  go aig.iter .empty (.emptyWithCapacity aig.size)
+where
+  go iter (state : Aig) (map : Array Lit)
+    (size : iter.var.idx = map.size := by grind)
+    (valid : ∀ {lit} (_ : lit ∈ map), lit.validIn state := by grind) :=
+    match h : iter.step.val with
+    | .skip it => go iter state map
+    | .done => state
+    | .yield it' var =>
+      let mapLit (lit : Lit) (h : lit.var < var := by grind) : Lit :=
+        map[lit.var.idx]'(by grind) |>.invert lit.inverted
+
+      let res : Aig × Lit := 
+        match h : aig[var]'(by grind) with
+        | .false => (state, .false)
+        | .input _ | .latch _ =>
+          let (eq:=_) (state, idx) := state.addInput
+          (state, idx.getLit state)
+        | .and rhs0 rhs1 => state.addAnd (mapLit rhs0) (mapLit rhs1)
+
+      go it' res.fst (map.push res.snd) (by simp; grind) (by simp [res]; grind)
+  termination_by iter.length
+  decreasing_by all_goals grind
